freeze

src/Bedrock/End2End/X25519/EdwardsXYZT.v
@@ -21,7 +21,6 @@ Require Import coqutil.Map.Interface.
 Require Import coqutil.Map.OfListWord.
 From coqutil.Tactics Require Import Tactics letexists eabstract rdelta reference_to_string ident_of_string.
 Require Import coqutil.Word.Bitwidth32.
-Require Import coqutil.Word.Bitwidth.
 Require Import coqutil.Word.Interface.
 Require Import coqutil.Word.Naive.
 From Coq Require Import Init.Byte.
@@ -160,6 +159,65 @@ Definition readd := func! (p_out, p_a, p_c) {
   fe25519_mul(p_out.Z, F, G)
 }.
 
+(* Size of a projective point in bytes. *)
+Local Notation pp_size := 200.
+(* Size of a cached point in bytes. *)
+Local Notation pc_size := 160.
+
+(* TODO I guess we can unify P256 and this one? *)
+Definition memcopy := func! (d, s, n) {
+  memmove(d, s, n)
+}.
+
+Definition copy_projective_point := func! (p_out, p_in) {
+  memcopy(p_out, p_in, $pp_size)
+}.
+
+Definition zero_projective_point := func! (zero) {
+  fe25519_from_word(zero.X, $0);
+  fe25519_from_word(zero.Y, $1);
+  fe25519_from_word(zero.Z, $1);
+  fe25519_from_word(zero.Ta, $0);
+  fe25519_from_word(zero.Tb, $1)
+}.
+
+(* Input is a projective point p, output is multiples of p as cached points, to be used for scalar multiplication. *)
+Definition cached_multiples := func! (p_ai, p_a, p_d) {
+  (* The first point is 0*A, so just zero. *)
+  stackalloc pp_size as zero;
+  zero_projective_point(zero);
+  to_cached(p_ai, zero, p_d);
+
+  (* The second point is 1*A.*)
+  to_cached(p_ai+$pc_size, p_a, p_d);
+
+  (* Helper array of normal points for double and add results, contains multiples of A. *)
+  stackalloc 8*pp_size as p_ai_uncached;
+  (* copy 1*A into the helper array at index 1. *)
+  copy_projective_point(p_ai_uncached+$pp_size, p_a);
+
+  (* Remaining points are generated in a loop. *)
+  i = $2;
+  stackalloc pp_size as temp;
+  while (i < $16) {
+    double(temp, p_ai_uncached+((i >> $2) * $pp_size)); (* Double (i/2)*A, now temp contains i*A. *)
+    to_cached(p_ai+(i*$pc_size), temp, p_d); (* copy temp to Ai *)
+    if (i < $8) {
+      (* Save i*A for later, at index i. *)
+      copy_projective_point(p_ai_uncached+(i*$pp_size), temp)
+    };
+    (* Now for the odd numbers, calculate (i+1)*A, store in temp. *)
+    readd(temp, p_a, p_ai+(i*$pc_size));
+    (* Store (i+1)*A in the result array. *)
+    to_cached(p_ai+((i+$1)*$pc_size), temp, p_d);
+    if (i < $7) {
+      (* Save (i+1)*A for later. *)
+      copy_projective_point(p_ai_uncached+((i+$1)*$pp_size), temp)
+    };
+    i = i + $2
+  }
+}.
+
 Section WithParameters.
   Context {two_lt_M: 2 < M_pos}.
   (* TODO: Can we provide actual values/proofs for these, rather than just sticking them in the context? *)
@@ -207,6 +265,12 @@ Local Notation m1add_precomputed_coordinates :=
            (field:=field)(char_ge_3:=char_ge_3)(Feq_dec:=F.eq_dec)
            (a:=a)(d:=d)(nonzero_a:=nonzero_a)(square_a:=square_a)(nonsquare_d:=nonsquare_d)
            (a_eq_minus1:=a_eq_minus1)).
+Local Notation multiples :=
+  (multiples(F:=F M_pos)(Feq:=Logic.eq)(Fzero:=F.zero)(Fone:=F.one)
+                  (Fopp:=F.opp)(Fadd:=F.add)(Fsub:=F.sub)(Fmul:=F.mul)(Finv:=F.inv)(Fdiv:=F.div)
+                  (field:=field)(char_ge_3:=char_ge_3)(Feq_dec:=F.eq_dec)
+                  (a:=a)(d:=d)(nonzero_a:=nonzero_a)(a_eq_minus1:=a_eq_minus1)
+                  (twice_d:=twice_d)(k_eq_2d:=k_eq_2d)(square_a:=square_a)(nonsquare_d:=nonsquare_d)). 
 
 Local Notation "p .+ n" := (word.add p (word.of_Z n)) (at level 50, format "p .+ n", left associativity).
 
@@ -298,6 +362,58 @@ Global Instance spec_of_readd : spec_of "readd" :=
           m' =* a_plus_c p5@ p_out * a_repr p5@ p_a * c_repr p4@ p_c * R
   }.
 
+Instance spec_of_copy_projective_point : spec_of "copy_projective_point" :=
+  fnspec! "copy_projective_point"
+    (p_out p_in : word) /
+    (a : point) (a_repr : projective_repr a) (out : list byte) (R : _ -> Prop), {
+      requires t m :=
+        m =* out $@ p_out * a_repr p5@ p_in * R /\
+        Datatypes.length out = Z.to_nat (pp_size);
+      ensures t' m' :=
+        t = t' /\
+        m' =* a_repr p5@ p_out * a_repr p5@ p_in * R
+  }.
+
+Local Notation zero := (zero(nonzero_a:=nonzero_a)).
+
+Instance spec_of_zero_projective_point : spec_of "zero_projective_point" :=
+  fnspec! "zero_projective_point"
+    (p_zero : word) /
+    (out : list byte) (R : _ -> Prop), {
+      requires t m :=
+        m =* out $@ p_zero * R /\
+        Datatypes.length out = Z.to_nat (pp_size);
+      ensures t' m' :=
+        t = t' /\
+        exists zero_repr: projective_repr (zero),
+          m' =* zero_repr p5@ p_zero * R
+    }.
+
+Definition cached_point (p : word) (a : cached) : map.rep -> Prop :=
+  Lift1Prop.ex1 (fun a_repr : cached_repr a => (a_repr p4@ p)).
+(* TODO find a nice way to deal with felem_size_in_bytes/words <-> 40/10 *)
+Definition cached_point_size_in_words := Eval lazy in 4 * felem_size_in_words. (* 40 *)
+
+Instance spec_of_cached_multiples : spec_of "cached_multiples" :=
+  fnspec! "cached_multiples"
+    (p_ai p_a p_d: word) /
+    (a : point) (a_repr : projective_repr a) (d1: felem) (out : list byte) (R : _ -> Prop), {
+      requires t m :=
+        m =* out $@ p_ai * a_repr p5@ p_a * FElem p_d d1 *  R /\
+        Datatypes.length out = Z.to_nat (16*pc_size) /\
+        d = feval d1 /\
+        bounded_by tight_bounds d1;
+      ensures t' m' :=
+        t = t' /\
+        m' =* (array cached_point (word.of_Z pc_size) p_ai (List.map m1_prep (multiples 16 a))) * a_repr p5@ p_a * FElem p_d d1 * R
+    }.
+    
+Local Instance spec_of_memcopy : spec_of "memcopy" :=
+  fnspec! "memcopy" (p_d p_s n : word) / (d s : list byte) R,
+  { requires t m := m =* d$@p_d * s$@p_s * R /\ List.length d = n :> Z /\ List.length s = n :> Z /\ n <= 2^31; (* I suppose.. *)
+    ensures t' m' := t' = t /\ m' =* s$@p_d * s$@p_s * R }.
+
+
 Local Instance spec_of_fe25519_square : spec_of "fe25519_square" := Field.spec_of_UnOp un_square.
 Local Instance spec_of_fe25519_mul : spec_of "fe25519_mul" := Field.spec_of_BinOp bin_mul.
 Local Instance spec_of_fe25519_add : spec_of "fe25519_add" := Field.spec_of_BinOp bin_add.
@@ -314,6 +430,9 @@ Local Arguments word.of_Z : simpl never.
 Local Arguments word.add : simpl never.
 
 Local Arguments feval : simpl never.
+
+(* This is way too large to be unfolded here. *)
+Local Opaque F.to_Z.
 
 Local Ltac destruct_points :=
   repeat match goal with
@@ -361,7 +480,8 @@ Local Ltac solve_mem :=
   end.
 
 Local Ltac single_step :=
-  repeat straightline; straightline_call; ssplit; try solve_mem; try solve_bounds.
+  repeat straightline; straightline_call; ssplit; try solve_mem; try solve_bounds;
+  (* solve simple preconditions *) try listZnWords; try assumption.
 
 (* Attempts to find anybytes terms in the goal and rewrites the first corresponding stack hypothesis to byte representation.
    straightline only supports deallocation for byte representation at the moment. *)
@@ -378,18 +498,221 @@ Ltac solve_deallocation :=
   end;
   repeat straightline.
 
-Ltac split_output_stack stack_var ptr_var num_points :=
-  match goal with
+Ltac split_stack stack_var ptr_var num :=
+  multimatch goal with
   | H : context[stack_var $@ ptr_var] |- _ =>
     split_stack_at_n_in stack_var ptr_var 40%nat H;
     split_stack_at_n_in (skipn 40 stack_var) (ptr_var.+40) 40%nat H;
     split_stack_at_n_in (skipn 80 stack_var) (ptr_var.+80) 40%nat H;
-    match num_points with
+    match num with
     | 4 => idtac
     | 5 =>
       split_stack_at_n_in (skipn 120 stack_var) (ptr_var.+120) 40%nat H
     end
   end.
+
+Require Import bedrock2.ArrayCasts.
+(* projective_repr -> list byte TODO: felem -> list byte should go into Field.v *)
+Definition projective_repr_to_list_byte {p} (r : projective_repr p) : list byte :=
+  let '(x, y, z, ta, tb) := proj1_sig r in (ws2bs 4%nat x) ++ (ws2bs 4%nat y) ++ (ws2bs 4%nat z) ++ (ws2bs 4%nat ta) ++ (ws2bs 4%nat tb).
+
+
+(* r p5@ p -> (projective_repr_to_list_byte c) @$ p *)                              
+Lemma p5_impl_bytes : forall {p} (r : projective_repr p) p_r, 
+  Lift1Prop.impl1 (r p5@ p_r) ((projective_repr_to_list_byte r) $@ p_r).
+Proof.
+  intros.
+  destruct_points.
+  cbv [FElem Bignum.Bignum projective_repr_to_list_byte proj1_sig].
+  intros m H. extract_ex1_and_emp_in_hyps.
+  unshelve (erewrite <- (array1_iff_eq_of_list_word_at _ _ _ _)).
+  { change felem_size_in_words with 10%nat in *.
+    rewrite !List.length_app, !ws2bs_length. lia. }
+    
+  repeat (epose (array_append _ _ _ _ _) as i;
+  seprewrite0 i;
+  clear i).
+
+  repeat (
+  epose (iff1_sym (bytes_of_words _ _)) as B;
+  cbv [bytes_per] in B;
+  change (bytes_per_word 32) with 4 in *;
+  change (Z.to_nat 4) with 4%nat in *;
+  seprewrite0 B;
+  clear B).
+
+  change (Z.of_nat 4) with 4.
+  rewrite !ws2bs_length, !H_emp0, !H_emp1, !H_emp2, !H_emp3.
+  change felem_size_in_words with 10%nat.
+  bottom_up_simpl_in_goal. bottom_up_simpl_in_hyp H.
+  ecancel_assumption.
+Qed.
+
+(* p5@ -> $@, I want to match on p5@ but I don't know how *)
+Hint Extern 1 (Lift1Prop.impl1 (_) (sepclause_of_map (_ $@ ?p))) => (apply p5_impl_bytes) : ecancel_impl.
+
+Lemma bytes_impl_p5 : forall {p} (r : projective_repr p) p_r, 
+  Lift1Prop.impl1 ((projective_repr_to_list_byte r) $@ p_r) (r p5@ p_r).
+Proof.
+  intros.
+  destruct_points.
+  intros m H. cbv [projective_repr_to_list_byte proj1_sig] in *. 
+Admitted. (* I would need a length assumption somewhere. *)
+
+
+Lemma copy_projective_point_ok: program_logic_goal_for_function! copy_projective_point.
+Proof.
+  do 4 straightline.
+
+  repeat straightline.
+  straightline_call. ssplit.
+  { ecancel_assumption_impl. }
+  { ZnWords. }
+  { destruct_points. 
+    cbv [projective_repr_to_list_byte proj1_sig].
+    rewrite !length_app, !ws2bs_length.
+    cbv [FElem Bignum.Bignum] in *.  (* super weird that the length of felems is only guaranteed by FElem *)
+    extract_ex1_and_emp_in H0.
+    rewrite !H0_emp0, !H0_emp1, !H0_emp2, !H0_emp3, H0_emp4.
+    change felem_size_in_words with 10%nat.
+    ZnWords. }
+  { ZnWords. }
+   
+  repeat straightline.
+  
+  (* getting the lengths here is very annoyting, this should be inherent to felem, and not just in FElem. *)
+  (* this is essentially the backwards direction of p5_impl_bytes, but with lengths from assumptions *)
+  destruct_points. cbv [projective_repr_to_list_byte proj1_sig FElem Bignum.Bignum] in *.
+  extract_ex1_and_emp_in_hyps. extract_ex1_and_emp_in_goal. ssplit; try assumption.
+
+  (* TODO figure out how to do with with seprewrite directly, or create a tactic/lemma. *)
+  repeat (epose ((bytes_of_words _ _)) as B;
+  cbv [bytes_per] in B;
+  change (bytes_per_word 32) with 4 in *;
+  change (Z.to_nat 4) with 4%nat in *;
+  change (Z.of_nat 4) with 4 in *; 
+  seprewrite0 B;
+  clear B).
+
+  assert (Z.of_nat (Datatypes.length (ws2bs 4 f2 ++ ws2bs 4 f3 ++ ws2bs 4 f1 ++ ws2bs 4 f0 ++ ws2bs 4 f)) <= 2 ^ 32).
+  {
+     rewrite !List.length_app, !ws2bs_length, !H0_emp0, !H0_emp1, !H0_emp2, !H0_emp3, !H0_emp4.
+     change felem_size_in_words with 10%nat. lia. 
+  }
+  epose (iff1_sym (array1_iff_eq_of_list_word_at _ _ _)) as B.
+  seprewrite_in B H4.
+  clear B.
+  epose (iff1_sym (array1_iff_eq_of_list_word_at _ _ _)) as B.
+  seprewrite_in B H4.
+  clear B.
+  Unshelve. all: try assumption.
+
+  repeat (epose (array_append _ _ _ _ _) as B; seprewrite_in B H4; clear B).
+
+  rewrite !ws2bs_length, !H0_emp0, !H0_emp1, !H0_emp2, !H0_emp3 in *.
+  change felem_size_in_words with 10%nat in *.
+  bottom_up_simpl_in_goal. bottom_up_simpl_in_hyp H4.
+  ecancel_assumption.
+Qed.
+
+Lemma zero_projective_point_ok: program_logic_goal_for_function! zero_projective_point.
+Proof.
+  do 4 straightline.
+  
+  pose word32_ok. (* required to run listZnWords on goals without words but with nasty lists *)
+  split_stack out p_zero 5.
+  
+  repeat straightline.
+  repeat single_step.
+
+  repeat straightline.
+  unshelve eexists.
+  eexists (x, x0, x1, x2, x3); ssplit. (* TODO don't name these directly, if I can avoid it*)
+  cbv [zero coordinates proj1_sig]. rewrite H20, H17, H14, H11, H8. bottom_up_simpl_in_goal.
+  f_equal.
+  all: try solve_bounds.
+  cbv [coordinates proj1_sig].
+  ecancel_assumption_impl.
+Qed.
+
+  (* TODO if I could split the hirarchies and have functions that work on curve points 
+     and functions that work on field elements, I would probably have good time proving things,
+     cause I can always work on the same kind of thing in memory. splitting and reaggregating points
+     is quite annoying. that may also be caused by the sigma types in the representation though. *)
+Lemma cached_multiples_ok: program_logic_goal_for_function! cached_multiples.
+Proof.
+   (* Without this, resolution of cbv stalls out Qed. *)
+   (* TODO can't I mark these as opaque in this section and the locally, in a tactic unopaque them when needed. (Or opaque below, where the actual harm happens, which is probably modulo arithmetics.)*)
+  Strategy -1000 [un_xbounds bin_xbounds bin_ybounds un_square bin_mul bin_add bin_carry_add bin_sub bin_carry_sub un_outbounds bin_outbounds].
+
+
+  (* put zero into ai[0] *)
+  repeat straightline.
+  seprewrite_in array1_iff_eq_of_list_word_at H9; [lia|].
+  single_step.
+  repeat straightline.
+  split_stack_at_n_in out p_ai 160%nat H21. (* split out ai[0] *)
+  single_step.
+  
+  (* put A into ai[1] *)
+  repeat straightline.
+  split_stack_at_n_in (skipn 160 out) (p_ai.+160) 160%nat H22. (* split out ai[1]*)
+  single_step.
+
+  (* allocate helper array (and split it up here already? might make stuff slow) *)
+  repeat straightline.
+  seprewrite_in array1_iff_eq_of_list_word_at H23; [lia|]. (* because allocation uses array, best way is to build a switch for allocation to use $@. *)
+
+  (* copy over 1*A to p_ai_uncached *)
+  split_stack_at_n_in stack1 a4 200%nat H23. (* index 0 - unused*)
+  split_stack_at_n_in (skipn 200 stack1) (a4.+200) 200%nat H23. (* index 1, will now be filled *)
+  single_step.
+  repeat straightline. 
+
+  (* Loop! - not working yet, I need to understand this better. probably a good idea to try proving an easier loop first. *)
+  refine (let multiples_a := multiples 16 a0 in
+          let cached_multiples_a := List.map m1_prep multiples_a in
+          let uncached_multiples_a := List.firstn 8 multiples_a in
+          tailrec
+            (*ghosttypes*)([point; felem; map.rep -> Prop; list byte; list byte; projective_repr a0])
+            (*variables*)(["i"; "p_ai"; "p_a"; "p_d"; "p_ai_uncached"; "temp"])
+            (*spec*)(fun (v:Z) (ghosts:hlist [point; felem; map.rep -> Prop; list byte; list byte; projective_repr a]) =>
+              let '(a, d1, R, out, stack1, a_repr) := HList.tuple.of_list ghosts in
+              fun t m (vars:tuple word 6) =>
+                let '(i, p_ai, p_a, p_d, p_ai_uncached, temp) := vars in
+                let i_z := word.unsigned i in
+                PrimitivePair.pair.mk
+                  (* Invariant P *)
+                  (v = (8 - i_z / 2) /\
+                   i_z mod 2 = 0 /\ 2 <= i_z < 16 /\
+                   m =* array cached_point (word.of_Z pc_size) p_ai (List.firstn (Z.to_nat i_z) cached_multiples_a) *
+                        (skipn (Z.to_nat i_z * pc_size) out) $@ (p_ai .+ (i_z * pc_size)) *
+                        array projective_point (word.of_Z pp_size) p_ai_uncached (List.firstn (Z.to_nat (i_z/2)) uncached_multiples_a) *
+                        (skipn (Z.to_nat (i_z/2) * pp_size) stack1) $@ (p_ai_uncached .+ ((i_z/2) * pp_size)) *
+                        anybytes temp pp_size *
+                        a_repr p5@ p_a * FElem p_d d1 * R)
+                  (* Postcondition Schema Q *)
+                  (fun T_f M_f vars_f =>
+                     let '(i_f, p_ai_f, p_a_f, p_d_f, p_ai_uncached_f, temp_f) := vars_f in
+                     M_f =* array cached_point (word.of_Z pc_size) p_ai cached_multiples_a *
+                            a_repr p5@ p_a * FElem p_d d1 * R))
+            (*measure*)ltac:(exact Z.lt) _ _ _ _ _ _ _);
+  loop_simpl.
+
+  { (* Hpre: Invariant holds before loop *)
+    (* Prove that P holds for i=2 *)
+    admit. }
+  { (* Hwf: well-foundedness of lt *)
+    exact (Z.lt_wf _). }
+  { (* Hbody: Loop body preserves invariant and decreases measure *)
+    admit. }
+  { (* Hpost: Q implies function postcondition *)
+    admit. }
+  { (* Initial values for locals *)
+    admit. }
+  { (* Initial values for ghosts *)
+    admit. }
+
 
 Lemma to_cached_ok: program_logic_goal_for_function! to_cached.
 Proof.
